Definition of Model.t simplified

src/Decide.v
@@ -7,36 +7,36 @@ Require Model.
 Require NoDeps.
 Require Import Semantics.
 
-Fixpoint not_stuck {E S A} {m : Model.t E S} (dec : Model.Dec.t m) (s : S)
-  (x : Choose.t E A) : bool :=
+Fixpoint not_stuck {E S A} (m : Model.t E S) (s : S) (x : Choose.t E A)
+  : bool :=
   match x with
   | Choose.Ret _ => true
-  | Choose.Call c _ => if dec c s then true else false
-  | Choose.Choose x1 x2 => orb (not_stuck dec s x1) (not_stuck dec s x2)
+  | Choose.Call c _ =>
+    match m c s with
+    | Some _ => true
+    | None => false
+    end
+  | Choose.Choose x1 x2 => orb (not_stuck m s x1) (not_stuck m s x2)
   end.
 
-Fixpoint aux {E S A} {m : Model.t E S} (dec : Model.Dec.t m) (s : S)
-  (x : Choose.t E A) : bool :=
+Fixpoint aux {E S A} (m : Model.t E S) (s : S) (x : Choose.t E A) : bool :=
   match x with
   | Choose.Ret _ => true
   | Choose.Call c h =>
-    match dec c s with
-    | left H =>
-      let s' := Model.state m c s H in
-      let x' := h (Model.answer m c s H) in
-      andb (not_stuck dec s' x') (aux dec s' x')
-    | right _ => true
+    match m c s with
+    | Some (a, s') => andb (not_stuck m s' (h a)) (aux m s' (h a))
+    | None => true
     end
-  | Choose.Choose x1 x2 => andb (aux dec s x1) (aux dec s x2)
+  | Choose.Choose x1 x2 => andb (aux m s x1) (aux m s x2)
   end.
 
-Definition dead_lock_free {E S A} {m : Model.t E S} (dec : Model.Dec.t m)
-  (s : S) (x : Choose.t E A) : bool :=
-  andb (not_stuck dec s x) (aux dec s x).
+Definition dead_lock_free {E S A} (m : Model.t E S) (s : S) (x : Choose.t E A)
+  : bool :=
+  andb (not_stuck m s x) (aux m s x).
 
 Module Choose.
-  Fixpoint not_stuck_ok {E S A} {m : Model.t E S} {dec : Model.Dec.t m} {s : S}
-    {x : Choose.t E A} (H : not_stuck dec s x = true)
+  Fixpoint not_stuck_ok {E S A} {m : Model.t E S} {s : S} {x : Choose.t E A}
+    (H : not_stuck m s x = true)
     : (exists p, exists v, Choose.Last.Eval.t p x v) \/
       (exists c, exists x', exists s', Choose.Step.t m c s x x' s').
     destruct x as [v | c h | x1 x2]; simpl in H.
@@ -44,13 +44,17 @@ Module Choose.
       exists Choose.Path.Done, v.
       apply Choose.Last.Eval.Ret.
     - right.
-      destruct (dec c s) as [H_pre |].
-      + exists c, (h (Model.answer m c s H_pre)), (Model.state m c s H_pre).
-        apply (Choose.Step.New _ _ _ _ _ Choose.Path.Done).
-        apply Choose.Eval.Call.
-      + congruence.
+      case_eq (m c s).
+      + intros p H_m; destruct p as [a s'].
+        exists c, (h a), s'.
+        apply (Choose.Step.New _ _ _ _ _ Choose.Path.Done a s').
+        * exact H_m.
+        * apply Choose.Eval.Call.
+      + intro H_m.
+        rewrite H_m in H.
+        congruence.
     - destruct (orb_prop _ _ H) as [H_not_stuck | H_not_stuck].
-      + destruct (not_stuck_ok _ _ _ _ _ _ _ H_not_stuck) as
+      + destruct (not_stuck_ok _ _ _ _ _ _ H_not_stuck) as
         [[p [v H_last]] | [c [x' [s' H_step]]]].
         * left.
           eexists; eexists.
@@ -59,10 +63,10 @@ Module Choose.
         * right.
           exists c, x', s'.
           destruct H_step.
-          eapply Choose.Step.New.
+          eapply Choose.Step.New; [exact H0 |].
           apply Choose.Eval.ChooseLeft.
           exact H1.
-      + destruct (not_stuck_ok _ _ _ _ _ _ _ H_not_stuck) as
+      + destruct (not_stuck_ok _ _ _ _ _ _ H_not_stuck) as
         [[p [v H_last]] | [c [x' [s' H_step]]]].
         * left.
           eexists; eexists.
@@ -71,14 +75,14 @@ Module Choose.
         * right.
           exists c, x', s'.
           destruct H_step.
-          eapply Choose.Step.New.
+          eapply Choose.Step.New; [exact H0 |].
           apply Choose.Eval.ChooseRight.
           exact H1.
   Defined.
 
   Fixpoint dead_lock_free_ok_no_deps {X Y S A} {m : Model.t (NoDeps.E X Y) S}
-    (dec : Model.Dec.t m) {s : S} {x : Choose.t (NoDeps.E X Y) A}
-    (H : dead_lock_free dec s x = true) : Choose.DeadLockFree.t m s x.
+    {s : S} {x : Choose.t (NoDeps.E X Y) A} (H : dead_lock_free m s x = true)
+    : Choose.DeadLockFree.t m s x.
     destruct (proj1 (andb_true_iff _ _) H) as [H_not_stuck H_aux].
     destruct (not_stuck_ok H_not_stuck) as [[p [v H_v]] | [c [x' [s' H_x]]]].
     - now apply (Choose.DeadLockFree.Ret _ _ _ p v).
@@ -90,34 +94,30 @@ Module Choose.
       + inversion_clear H_x.
         inversion H1.
         rewrite <- H4 in *.
-        destruct (dec c' s) as [H_pre | H_not_pre]; simpl in H_aux.
-        * rewrite (Model.stable_state m c' s H0 H_pre).
-          rewrite (Model.stable_answer m c' s H0 H_pre).
-          now apply (dead_lock_free_ok_no_deps _ _ _ _ _ dec).
-        * destruct (H_not_pre H0).
+        rewrite H0 in H_aux.
+        now apply dead_lock_free_ok_no_deps.        
       + inversion_clear H_x.
         destruct (proj1 (andb_true_iff _ _) H_aux) as [H_x1 H_x2].
         inversion_clear H0.
         * apply (IHx1 H_x1 c').
-          eapply Choose.Step.New.
+          eapply Choose.Step.New; [exact H |].
           apply H1.
         * apply (IHx2 H_x2 c').
-          eapply Choose.Step.New.
+          eapply Choose.Step.New; [exact H |].
           apply H1.
   Qed.
 
-  Definition dead_lock_free_ok {E S A} {m : Model.t E S} (dec : Model.Dec.t m)
-    {s : S} {x : Choose.t E A} (H : dead_lock_free dec s x = true)
+  Definition dead_lock_free_ok {E S A} {m : Model.t E S} {s : S}
+    {x : Choose.t E A} (H : dead_lock_free m s x = true)
     : Choose.DeadLockFree.t m s x.
   Admitted.
 End Choose.
 
 Module C.
-  Definition dead_lock_free_ok {E S A} {m : Model.t E S} (dec : Model.Dec.t m)
-    {s : S} {x : C.t E A}
-    (H : dead_lock_free dec s (Compile.to_choose x) = true)
+  Definition dead_lock_free_ok {E S A} {m : Model.t E S} {s : S} {x : C.t E A}
+    (H : dead_lock_free m s (Compile.to_choose x) = true)
     : C.DeadLockFree.t m s x.
     apply Equiv.to_c.
-    now apply (Choose.dead_lock_free_ok dec).
+    now apply Choose.dead_lock_free_ok.
   Qed.
 End C.
