src/Examples/Locks.v
@@ -1,0 +1,2 @@
+(** * A finite number of global locks. *)
+
