src/Model.v
@@ -1,19 +1,4 @@
 Require Import Io.All.
 
-Record t (E : Effect.t) (S : Type) := New {
-  pre : Effect.command E -> S -> Prop;
-  answer : forall c s, pre c s -> Effect.answer E c;
-  state : forall c s, pre c s -> S;
-  stable_answer : forall c s H1 H2, answer c s H1 = answer c s H2;
-  stable_state : forall c s H1 H2, state c s H1 = state c s H2 }.
-Arguments New {E S} _ _ _ _ _.
-Arguments pre {E S} _ _ _.
-Arguments answer {E S} _ _ _ _.
-Arguments state {E S} _ _ _ _.
-Arguments stable_answer {E S} _ _ _ _ _.
-Arguments stable_state {E S} _ _ _ _ _.
-
-Module Dec.
-  Definition t {E S} (m : Model.t E S) : Type :=
-    forall c s, {Model.pre m c s} + {~ Model.pre m c s}.
-End Dec.
+Definition t (E : Effect.t) (S : Type) : Type :=
+  forall (c : Effect.command E), S -> option (Effect.answer E c * S).
